Generated/erc20shim/ERC20Shim/fun_balanceOf_user.lean
@@ -12,41 +12,36 @@ section
 open Clear EVMState Ast Expr Stmt FunctionDefinition State Interpreter ExecLemmas OutOfFuelLemmas Abstraction YulNotation PrimOps ReasoningPrinciple Utilities Generated.erc20shim ERC20Shim
 
 def A_fun_balanceOf (var : Identifier) (var_account : Literal) (s₀ s₉ : State) : Prop :=
-  ∀ erc20, balance_predicate erc20 s₀ → balance_predicate erc20 s₉
-
-  -- ∃ (s : State) (addr : UInt256), (s₉ = s⟦ var ↦ s.evm.sload addr ⟧)
+  let account := Address.ofUInt256 var_account
+  ∀ {erc20 : ERC20}, account ∈ erc20.balances →
+  ∀ bal_addr,
+  s₀.evm.keccak_map.lookup [ ↑account , ERC20Private.balances ] = some bal_addr →
+  erc20.balances.lookup account = some (s₀.evm.sload bal_addr) →
+  s₉[var]!! = s₀.evm.sload bal_addr
 
 lemma fun_balanceOf_abs_of_concrete {s₀ s₉ : State} {var var_account} :
   Spec (fun_balanceOf_concrete_of_code.1 var var_account) s₀ s₉ →
   Spec (A_fun_balanceOf var var_account) s₀ s₉ := by
-  unfold fun_balanceOf_concrete_of_code A_fun_balanceOf  
+  unfold fun_balanceOf_concrete_of_code A_fun_balanceOf
+
   rcases s₀ with ⟨evm, varstore⟩ | _ | _ <;> [simp only; aesop_spec; aesop_spec]
   apply spec_eq
   clr_funargs
 
-  intro hasFuel index_access erc20 pred_s₀
+  intro hasFuel ⟨s, keccak, prog⟩ erc20 hasBal bal_addr hasAddr loadAddr
+  clr_varstore
 
-  rcases index_access with ⟨sₖ, mapping, h'⟩
-  -- clr_spec at mapping
-
-  -- have sₖ_isOk : isOk sₖ := mapping_of_ok mapping (by simp)
-  -- rcases sₖ with ⟨evmₖ, _⟩ | _ | _ <;> try contradiction
-  -- use (Ok evmₖ varstore)
-
-  -- simp at *
-  -- rw [ ← State.insert_of_ok, ← State.insert_of_ok
-  --    , State.lookup_insert
-  --    ] at h'
-  -- symm at h'
-
-  -- by_cases h : evmₖ.hash_collision = true
-  -- · use 0
-  --   rw [ lookup_addr_fail mapping h] at h'
-  --   assumption
-  -- · rcases lookup_addr_ok mapping (by aesop) with ⟨addr, lookup_eq_addr⟩
-  --   use addr
-  --   rw [ lookup_eq_addr ] at h'
-  --   assumption
+  unfold A_mapping_index_access_mapping_address_uint256_of_address at keccak
+  simp at keccak
+  clr_spec at keccak
+  
+  obtain ⟨is_ok, lookup⟩ := keccak hasBal bal_addr hasAddr
+  obtain ⟨evmₛ, varstareₛ, ok_state⟩ := State_of_isOk is_ok
+  rw [lookup, ok_state] at prog
+  rw [← prog]
+  
+  unfold State.lookup!
+  simp
 
 end
 
